# Factoring

## Formulas

\[
  \begin{aligned}
    x^2 - (r+s)x + rs &= (x-r)(x-s)                                                             \h4 \\
    x^2 + 2ax + a^2 &= (x+a)^2                                                                  \h4 \\
    x^2 - 2ax + a^2 &= (x-a)^2                                                                  \h4 \\[1em]
    a^2 - b^2 &= (a - b)(a + b)                            && \text{Difference of squares}      \h4 \\
    a^3 - b^3 &= (a - b)(a^2 + ab + b^2)                   && \text{Difference of cubes}        \h4 \\
    a^4 - b^4 &= (a^2-b^2)(a^2+b^2) = (a-b)(a+b)(a^2+b^2)  && \text{Difference of tesseracts?}  \h4 \\
    a^n - b^n &= (a - b)(a^{n-1}b^0 + a^{n-2}b^1 + \ldots + a^1b^{n-2} + a^0b^{n-1})            \h4 \\[1em]
    a^2 + b^2 &= (a - bi)(a + bi)                          && \text{Sum of squares (imaginary)} \h4 \\
    a^3 + b^3 &= (a + b)(a^2 - ab + b^2)                   && \text{Sum of cubes}               \h4 \\
    a^4 + b^4 &= (a^2-\sqrt{2}ab+b^2)(a^2+\sqrt{2}ab+b^2)  && \text{Sum of tesseracts?}         \h4 \\
    a^n + b^n &= (a + b)(a^{n-1}b^0 - a^{n-2}b^1 + \ldots - a^1b^{n-2} + a^0b^{n-1}) && n \text{ must be odd} \h4 \\
  \end{aligned}
\]

## Quadratic Formula

\[
  x = {-b \pm \sqrt{b^2 - 4ac} \over 2a}
\]
