# Rationals

## Rules

\[
  \begin{aligned}
    a^{-1} &= {1 \over a  }                                   \h7 \\
    a^{-n} &= {1 \over a^n}                                   \h7 \\[1em]
    \bigg({a \over b}\bigg)^{-1} &=       {b \over a}         \h7 \\
    \bigg({a \over b}\bigg)^{-n} &= \bigg({b \over a}\bigg)^n \h7 \\[1em]
    { 1          \over {a \over b}} &= { b \over a}           \h7 \\
    { c          \over {a \over b}} &= {cb \over a }          \h7 \\
    {{a \over b} \over  c         } &= {a  \over cb}          \h7 \\
  \end{aligned}
\]
